

Chapter 6-3

1-21 odd

In Problems 1-14 for each differential equation find two linearly independent power series solutions about the ordinary point $x=0$.

1. $y'' = xy$
2. $y'' - 2xy' + y = 0$
3. $y'' + x^2y' + xy = 0$
4. $(x-1)y'' + y' = 0$
5. $(x^2-1)y'' + 4xy' + 2y = 0$
6. $(x^2+2)y'' + 3xy' - y = 0$
7. $y'' - (x+1)y' - y = 0$

In Problems 15-18 use the power series method to solve the given differential equation subject to the indicated initial conditions.

15. $(x-1)y'' - xy' + y = 0, \quad y(0) = -2, y'(0) = 6$
16. $y'' - 2xy' + 8y = 0, \quad y(0) = 3, y'(0) = 0$

In Problems 19-22 use the procedure illustrated in Example 9 to find two power series solutions of the given differential equation about the ordinary point $x = 0$.

19. $y'' + (\sin x)y = 0$
20. $y'' + e^{-x}y = 0$

Answers

$$1. \quad y_1(x) = c_0 \left[1 + \frac{1}{3 \cdot 2} x^3 + \frac{1}{6 \cdot 5 \cdot 3 \cdot 2} x^6 + \frac{1}{9 \cdot 8 \cdot 6 \cdot 5 \cdot 3 \cdot 2} x^9 + \dots \right]$$

$$y_2(x) = c_1 \left[x + \frac{1}{4 \cdot 3} x^4 + \frac{1}{7 \cdot 6 \cdot 4 \cdot 3} x^7 + \dots \right]$$

2.

$$y_1(x) = c_0 \left[1 - \frac{1}{27} x^3 - \frac{3}{4!} x^4 - \frac{21}{6!} x^6 - \dots \right]$$

$$y_2(x) = c_1 \left[x + \left(\frac{1}{3!} x^3 + \frac{5}{5!} x^5 + \frac{45}{7!} x^7 + \dots \right) \right]$$

$$3. \quad y_1(x) = c_0 \left[1 - \frac{1}{3!} x^3 + \frac{4^2}{6!} x^6 - \frac{7^2 \cdot 4^2}{9!} x^9 + \dots \right]$$

$$y_2(x) = c_1 \left[x - \frac{2^2}{4!} x^4 + \frac{5^2 \cdot 2^2}{7!} x^7 - \frac{8^2 \cdot 5^2 \cdot 2^2}{10!} x^{10} + \dots \right]$$

$$4. \quad y_1(x) = c_0; \quad y_2(x) = c_1 \sum_{n=1}^{\infty} \frac{1}{n} x^n$$

$$5. \quad y_1(x) = c_0 \sum_{n=0}^{\infty} x^{2n}; \quad y_2(x) = c_1 \sum_{n=0}^{\infty} x^{2n+1}$$

$$6. \quad y_1(x) = c_0 \left[1 + \frac{x^2}{4} - \frac{7}{4 \cdot 4!} x^4 + \frac{23 \cdot 7}{8 \cdot 6!} x^6 - \dots \right]$$

$$y_2(x) = c_1 \left[x - \left(\frac{1}{6} x^3 + \frac{14}{2 \cdot 5!} x^5 - \frac{34 \cdot 14}{4 \cdot 7!} x^7 - \dots \right) \right]$$

$$7. \quad y_1(x) = c_0 \left[1 + \frac{\frac{1}{2} x^2}{x^2} + \frac{\frac{1}{3!} x^3}{x^3} + \frac{\frac{1}{4!} x^4}{x^4} + \dots \right]$$

$$y_2(x) = c_1 \left[x + \frac{1}{2!} x^2 + \frac{1}{3!} x^3 + \frac{1}{4!} x^4 + \dots \right]$$

$$8. \quad y(x) = -2 \left[1 + \frac{1}{2!} x^2 + \frac{1}{3!} x^3 + \frac{1}{4!} x^4 + \dots \right] + 6x$$

$$= 8x - 2e^x$$

$$9. \quad y(x) = 3 - 12x^2 + 4x^4$$

$$10. \quad y_1(x) = c_0 \left[1 - \frac{\frac{1}{6} x^3}{x^3} + \frac{1}{120} x^5 + \dots \right]$$

$$y_2(x) = c_1 \left[x - \frac{1}{12} x^4 + \frac{1}{180} x^6 + \dots \right]$$

$$11. \quad y_1(x) = c_0 \left[1 - \frac{x^2}{6} + \frac{x^3}{6} - \frac{x^4}{40} + \dots \right]$$